Cslib.lean
@@ -288,6 +288,7 @@ public import Cslib.Logics.Bimodal.Theorems.TemporalDerived
 public import Cslib.Logics.HML.Basic
 public import Cslib.Logics.HML.LogicalEquivalence
 public import Cslib.Logics.LTL.Embedding
+public import Cslib.Logics.LTL.ModelChecking
 public import Cslib.Logics.LTL.Semantics.GNBA
 public import Cslib.Logics.LTL.Semantics.OmegaExecutionSatisfies
 public import Cslib.Logics.LTL.Semantics.OmegaRegular
